theories/steps.v
@@ -92,10 +92,11 @@ Proof.
   intros Eq. by destruct (foldr_gmap_insert_lookup _ _ _ _ _ _ Eq).
 Qed.
 
-Lemma alloc_step_wf σ σ' e e' l bor T amod:
-  base_step e σ.(cheap) (Some $ AllocEvt l bor T amod) e' σ'.(cheap) [] →
-  instrumented_step σ.(cheap) σ.(cstk) σ.(cbar) σ.(cclk)
-                    (Some $ AllocEvt l bor T amod)
+(** Alloc *)
+Lemma alloc_step_wf σ σ' e e' efs h0 l bor T:
+  base_step e σ.(cheap) (Some $ AllocEvt l bor T) e' h0 efs →
+  instrumented_step h0 σ.(cstk) σ.(cbar) σ.(cclk)
+                    (Some $ AllocEvt l bor T)
                   σ'.(cheap) σ'.(cstk) σ'.(cbar) σ'.(cclk) →
   Wf σ → Wf σ'.
 Proof.
@@ -104,10 +105,6 @@ Proof.
   intros BS IS WF. inversion BS. clear BS. simplify_eq.
   destruct (tsize T) eqn:Eqs.
   - inversion IS; clear IS; simplify_eq; constructor; simpl.
-    + rewrite Eqs /=. apply WF.
-    + apply WF.
-    + rewrite Eqs /=. apply WF.
-    + rewrite Eqs /=. apply WF.
     + rewrite Eqs /=. apply WF.
     + move => ?? bor /(state_wf_mem_bor _ WF).
       destruct bor as [|[]]; simpl; lia.
@@ -118,17 +115,6 @@ Proof.
       move => ?? si Eq In. move : (state_wf_stack_item _ WF _ _ _ Eq In).
       destruct si; [simpl; lia|done..].
   - inversion IS; clear IS; simplify_eq; constructor; cbn -[ init_mem].
-    + rewrite Eqs init_stacks_foldr init_mem_foldr. apply foldr_gmap_insert_dom, WF.
-    + intros l1 l2 bor. rewrite init_mem_foldr.
-      intros [|Eq]%foldr_gmap_insert_lookup; [done|].
-      by apply (state_wf_mem_bor _ WF _ _ _ Eq).
-    + intros l1 stack. rewrite init_stacks_foldr.
-      intros [->|Eq]%foldr_gmap_insert_lookup; [done|].
-      by apply (state_wf_stack_frozen _ WF _ _ Eq).
-    + intros l1 stack si. rewrite init_stacks_foldr.
-      intros [->|Eq]%foldr_gmap_insert_lookup.
-      * by intros ->%elem_of_list_singleton.
-      * by apply (state_wf_stack_item _ WF _ _ _ Eq).
     + rewrite Eqs init_stacks_foldr init_mem_foldr. apply foldr_gmap_insert_dom, WF.
     + intros l1 l2 bor. rewrite init_mem_foldr.
       intros [|Eq]%foldr_gmap_insert_lookup; [done|].
@@ -161,14 +147,13 @@ Lemma accessN_dealloc_delete' α β l bor n α' (m: nat):
   α' = fold_right (λ (i: nat) α, delete (l +ₗ i) α) α (seq m n).
 Proof.
   revert α.
-  induction n as [|n IHn]; intros α; [by move => [->]|].
-  rewrite /accessN. case_match; [|done].
-  case_match; [|done].
-  move => /IHn ->. clear. revert α m. induction n; intros α m.
+  induction n as [|n IHn]; intros α; [by move => [->]|]. simpl.
+  case lookup => stack /= ; [|done]. case access1 => stack'; [|done].
+  move => /IHn ->. clear. revert α m. induction n as [|n IH]; intros α m.
   - by rewrite /= shift_loc_0.
   - simpl. f_equal.
     by rewrite shift_loc_assoc -Nat2Z.inj_add -Nat.add_succ_comm Nat2Z.inj_add
-               -shift_loc_assoc IHn.
+               -shift_loc_assoc IH.
 Qed.
 Lemma accessN_dealloc_delete α β l bor n α':
   accessN α β l bor n AccessDealloc = Some α' →
@@ -185,16 +170,17 @@ Proof.
   by rewrite 2!dom_delete IHcs.
 Qed.
 
-Lemma dealloc_step_wf σ σ' e e' l bor T:
-  base_step e σ.(cheap) (Some $ DeallocEvt l bor T) e' σ'.(cheap) [] →
-  instrumented_step σ.(cheap) σ.(cstk) σ.(cbar) σ.(cclk)
+(** Dealloc *)
+Lemma dealloc_step_wf σ σ' e e' efs h0 l bor T :
+  base_step e σ.(cheap) (Some $ DeallocEvt l bor T) e' h0 efs →
+  instrumented_step h0 σ.(cstk) σ.(cbar) σ.(cclk)
                     (Some $ DeallocEvt l bor T)
                   σ'.(cheap) σ'.(cstk) σ'.(cbar) σ'.(cclk) →
   Wf σ → Wf σ'.
 Proof.
-  destruct σ as [h stk bar clk].
-  destruct σ' as [h' stk' bar' clk']. simpl.
-  intros BS IS WF. inversion BS. clear BS. simplify_eq.
+  destruct σ as [h stk bar clk]. destruct σ' as [h' stk' bar' clk']. simpl.
+  intros BS IS WF.
+  inversion BS. clear BS. simplify_eq.
   inversion IS. clear IS. simplify_eq.
   rewrite (accessN_dealloc_delete stk bar' l bor (tsize T) stk'); [|done].
   constructor; simpl.
@@ -207,3 +193,176 @@ Proof.
   - intros ??? Eq%foldr_gmap_delete_lookup.
     apply (state_wf_stack_item _ WF _ _ _ Eq).
 Qed.
+
+(** Copy *)
+
+Lemma dom_map_insert_is_Some `{FinMapDom K M D} {A} (m : M A) i x :
+  is_Some (m !! i) → dom D (<[i:=x]>m) ≡ dom D m.
+Proof.
+  intros IS. rewrite dom_insert. apply (anti_symm (⊆)).
+  - apply union_least; [|done]. by apply elem_of_subseteq_singleton, elem_of_dom.
+  - by apply union_subseteq_r.
+Qed.
+
+Lemma accessN_normal_dom α β l bor n kind α' (ND: kind ≠ AccessDealloc) :
+  accessN α β l bor n kind = Some α' →
+  dom (gset loc) α ≡ dom (gset loc) α'.
+Proof.
+  revert α α'. induction n as [|n IH]; intros α α'; [by move => /= [-> //]|].
+  simpl. destruct (α !! (l +ₗ n)) eqn:Eq; [|done].
+  simpl. case access1 => stack' /=; [|done]. intros Eq2.
+  have Eq3: dom (gset loc) α' ≡ dom (gset loc) (<[l +ₗ n:=stack']> α).
+  { destruct kind; [..|done]; move : Eq2 => /IH <- //. } clear Eq2.
+  rewrite Eq3. symmetry. apply dom_map_insert_is_Some. by eexists.
+Qed.
+
+Lemma copy_step_wf σ σ' e e' efs h0 l bor T :
+  base_step e σ.(cheap) (Some $ CopyEvt l bor T) e' h0 efs →
+  instrumented_step h0 σ.(cstk) σ.(cbar) σ.(cclk)
+                    (Some $ CopyEvt l bor T)
+                  σ'.(cheap) σ'.(cstk) σ'.(cbar) σ'.(cclk) →
+  Wf σ → Wf σ'.
+Proof.
+  destruct σ as [h stk bar clk]. destruct σ' as [h' stk' bar' clk']. simpl.
+  intros BS IS WF.
+  inversion BS. clear BS. simplify_eq.
+  inversion IS. clear IS. simplify_eq.
+  constructor; simpl.
+  - rewrite -(accessN_normal_dom stk bar' l bor (tsize T) AccessRead);
+      [by apply WF|done..].
+  - apply WF.
+  - admit. (* stk' sub of stk *)
+  - admit. (* stk' sub of stk *)
+Abort.
+
+(** Write *)
+
+Lemma write_mem_dom l vl h
+  (DEFINED: ∀ i : nat, (i < strings.length vl)%nat → is_Some (h !! (l +ₗ i))) :
+  dom (gset loc) (write_mem l vl h) ≡ dom (gset loc) h.
+Proof.
+  revert l h DEFINED. induction vl as [|v vl IH]; intros l h DEFINED; [done|].
+  rewrite /= IH.
+  - apply dom_map_insert_is_Some. rewrite -(shift_loc_0_nat l).
+    apply DEFINED. simpl. lia.
+  - intros i Lt. rewrite lookup_insert_is_Some'. right.
+    rewrite (shift_loc_assoc_nat l 1). apply DEFINED. simpl. lia.
+Qed.
+
+Lemma write_step_wf σ σ' e e' efs h0 l bor T :
+  base_step e σ.(cheap) (Some $ WriteEvt l bor T) e' h0 efs →
+  instrumented_step h0 σ.(cstk) σ.(cbar) σ.(cclk)
+                    (Some $ WriteEvt l bor T)
+                  σ'.(cheap) σ'.(cstk) σ'.(cbar) σ'.(cclk) →
+  Wf σ → Wf σ'.
+Proof.
+  destruct σ as [h stk bar clk]. destruct σ' as [h' stk' bar' clk']. simpl.
+  intros BS IS WF.
+  inversion BS. clear BS. simplify_eq.
+  inversion IS. clear IS. simplify_eq.
+  constructor; simpl.
+  - rewrite -(accessN_normal_dom stk bar' l bor (tsize T) AccessWrite);
+      [|done..].
+    rewrite write_mem_dom; [by apply WF|done].
+  - admit. (* only true if whatever in el is bound in the memory *)
+  - admit. (* stk' sub of stk *)
+  - admit. (* stk' sub of stk *)
+Abort.
+
+(** Deref *)
+Lemma deref_step_wf σ σ' e e' efs h0 l bor T mut :
+  base_step e σ.(cheap) (Some $ DerefEvt l bor T mut) e' h0 efs →
+  instrumented_step h0 σ.(cstk) σ.(cbar) σ.(cclk)
+                    (Some $ DerefEvt l bor T mut)
+                  σ'.(cheap) σ'.(cstk) σ'.(cbar) σ'.(cclk) →
+  Wf σ → Wf σ'.
+Proof.
+  destruct σ as [h stk bar clk]. destruct σ' as [h' stk' bar' clk']. simpl.
+  intros BS IS WF.
+  inversion BS. clear BS. simplify_eq.
+  inversion IS. clear IS. simplify_eq.
+  constructor; simpl; apply WF.
+Qed.
+
+(** NewCall *)
+Lemma newcall_step_wf σ σ' e e' efs h0 n :
+  base_step e σ.(cheap) (Some $ NewCallEvt n) e' h0 efs →
+  instrumented_step h0 σ.(cstk) σ.(cbar) σ.(cclk)
+                    (Some $ NewCallEvt n)
+                  σ'.(cheap) σ'.(cstk) σ'.(cbar) σ'.(cclk) →
+  Wf σ → Wf σ'.
+Proof.
+  destruct σ as [h stk bar clk]. destruct σ' as [h' stk' bar' clk']. simpl.
+  intros BS IS WF.
+  inversion BS. clear BS. simplify_eq.
+  inversion IS. clear IS. simplify_eq.
+  constructor; simpl; [apply WF..|].
+  intros ??? Eq In. have SI := state_wf_stack_item _ WF _ _ _ Eq In.
+  destruct si; [done..|]. rewrite lookup_insert_is_Some'. by right.
+Qed.
+
+(** EndCall *)
+Lemma endcall_step_wf σ σ' e e' efs h0 n :
+  base_step e σ.(cheap) (Some $ EndCallEvt n) e' h0 efs →
+  instrumented_step h0 σ.(cstk) σ.(cbar) σ.(cclk)
+                    (Some $ EndCallEvt n)
+                  σ'.(cheap) σ'.(cstk) σ'.(cbar) σ'.(cclk) →
+  Wf σ → Wf σ'.
+Proof.
+  destruct σ as [h stk bar clk]. destruct σ' as [h' stk' bar' clk']. simpl.
+  intros BS IS WF.
+  inversion BS. clear BS. simplify_eq.
+  inversion IS. clear IS. simplify_eq.
+  constructor; simpl; [apply WF..|].
+  intros ??? Eq In. have SI := state_wf_stack_item _ WF _ _ _ Eq In.
+  destruct si; [done..|]. rewrite lookup_insert_is_Some'. by right.
+Qed.
+
+
+(** Retag *)
+Lemma retag_step_wf σ σ' e e' efs h0 l T kind :
+  base_step e σ.(cheap) (Some $ RetagEvt l T kind) e' h0 efs →
+  instrumented_step h0 σ.(cstk) σ.(cbar) σ.(cclk)
+                    (Some $ RetagEvt l T kind)
+                  σ'.(cheap) σ'.(cstk) σ'.(cbar) σ'.(cclk) →
+  Wf σ → Wf σ'.
+Proof.
+  destruct σ as [h stk bar clk]. destruct σ' as [h' stk' bar' clk']. simpl.
+  intros BS IS WF.
+  inversion BS. clear BS. simplify_eq.
+  inversion IS. clear IS. simplify_eq.
+  constructor; simpl.
+  - admit. (* no change in dom of h' stk' *)
+  - admit. (* new bor comes from increasing clk *)
+  - admit. (* new bor comes from increasing clk *)
+  - admit. (* barrier must be in memory *)
+Abort.
+
+(** None event step *)
+Lemma None_step_wf σ σ' e e' efs h0 :
+  base_step e σ.(cheap) None e' h0 efs →
+  instrumented_step h0 σ.(cstk) σ.(cbar) σ.(cclk)
+                    None
+                  σ'.(cheap) σ'.(cstk) σ'.(cbar) σ'.(cclk) →
+  Wf σ → Wf σ'.
+Proof.
+  destruct σ as [h stk bar clk]. destruct σ' as [h' stk' bar' clk']. simpl.
+  intros BS IS WF.
+  inversion BS; clear BS; simplify_eq;
+  inversion IS; clear IS; simplify_eq; apply WF.
+Qed.
+
+Lemma head_step_wf σ σ' e e' efs :
+  head_step e σ [] e' σ' efs → Wf σ → Wf σ'.
+Proof.
+  intros HS WF. inversion HS. simplify_eq. destruct oevent as [[]|].
+  - eapply alloc_step_wf; eauto.
+  - eapply dealloc_step_wf; eauto.
+  - admit.
+  - admit.
+  - eapply deref_step_wf; eauto.
+  - eapply newcall_step_wf; eauto.
+  - eapply endcall_step_wf; eauto.
+  - admit.
+  - eapply None_step_wf; eauto.
+Abort.
